glue is donegit add hol/bdd_test_casesScript.sml hol/table_arith_to_intervalScript.sml!

hol/bdd_test_casesScript.sml
@@ -30,10 +30,11 @@ open bdd_isomorphTheory;
 open bdd_end_to_endTheory;     
 
 open policy_arith_to_varTheory;
-
+open table_var_to_arithTheory;
 open table_arith_to_intervalTheory;
 
-
+open bdd_auxTheory;
+open table_bs_propertiesTheory;
      
 
 
@@ -78,16 +79,24 @@ val _ = type_abbrev("arith_policy_typ", “:((string# num list) action_expr) ari
 
 (* policy 1: arith POLICY representation *)
 
+val test_pd_type1 = “[("h" , type_record [("ttl", type_length 8);
+                                          ("flag", type_length 4)])]”;
+
+                                          
 val is_high_ttl = “(arithm_le (lv_acc (lv_x "h") "ttl") ^(BDDUtils.make_bv 100 8) )”;
 val is_low_ttl = “(arithm_ge (lv_acc (lv_x "h") "ttl") ^(BDDUtils.make_bv 1 8) )”;
 val is_flag_ok = “(arithm_le (lv_acc (lv_x "h") "flag") ^(BDDUtils.make_bv 3 4) )”;
 
         
 val policy1_me1 =   “[("x", ^is_high_ttl);
-                   ("y", ^is_low_ttl );
-                   ("z", ^is_flag_ok)]”;
+                      ("y", ^is_low_ttl );
+                      ("z", ^is_flag_ok)]”;
 
+val policy1_full_order = “[("a",["x";"y"]);("b",["z"])]”;                      
 
+val policy1_order = “["x";"y";"z"]”;                      
+
+    
 val arith_policy1_rule1 = “(arith_and (arith_a ^is_high_ttl) ( arith_a ^is_low_ttl) ,
                             action ("fwd",[(1:num)])):((string# num list) action_expr) arith_rule”;
                             
@@ -97,10 +106,12 @@ val arith_policy1_rule2 = “(arith_a (^is_flag_ok) , action ("fwd",[2]))
 val arith_policy1_rule3 = “(arith_a a_True, action ("drop",[])):((string# num list) action_expr) arith_rule”;
                     
 
-val arith_policy1 =   “[ ^arith_policy1_rule1 ;
+val arith_policy1 =   “[^arith_policy1_rule1 ;
                         ^arith_policy1_rule2 ;
                         ^arith_policy1_rule3]:((string# num list) action_expr) arith_policy”;
 
+
+                        
 val arith_policy1_eval = EVAL “convert_arith_to_var_policy ^arith_policy1 ^policy1_me1”;
 
 
@@ -126,19 +137,21 @@ val arith_policy1_var_policy1_thm = REWRITE_RULE[all_distinct_conj, arith_policy
 
         
 (* policy 1: var POLICY representation *)
-   
+(*   
 val var_policy1_rule1 = ``(And (Var "x") (Var "y"), action ("fwd",[1])): action_rule_type``;
 val var_policy1_rule2 = ``(Var "z", action ("fwd",[2])): action_rule_type``;
 val var_policy1_rule3 = ``(True, action ("drop",[])): action_rule_type``;
 
+
 val var_policy1 = ``[^var_policy1_rule1; ^var_policy1_rule2; ^var_policy1_rule3 ] : action_policy_type``;
+*)
 
 val eval_policy1_full_opt = EVAL ``mk_BDDPred_opt policy_structure (0,[],[(0, non_termn (NONE, ^var_policy1))]) [] ["x";"y";"z"] 1``;
 val eval_policy1_full_opt_rhs = optionSyntax.dest_some (rhs (concl eval_policy1_full_opt));
 
 
 (* automatically generate a table*)
-val test_groupings1 = rhs(concl(EVAL “[("a",["x";"y"]);("b",["z"])]”));
+val test_groupings1 = rhs(concl(EVAL policy1_full_order));
 val test_action_table1_auto = BDDUtils.bdd_to_tables_iterative eval_policy1_full_opt_rhs test_groupings1;
 
 (* now create a BDD for the table*)    
@@ -159,24 +172,487 @@ val policy1_thm = SIMP_RULE bool_ss [correct_var_policy_var_tables_exec_thm1] po
 
 val only_var_table1 = fst (dest_pair test_action_table1_auto);
    
-val test_pd_type1 = “[("h" , type_record [("ttl", type_length 8);
-                                          ("flag", type_length 4)])]”;
                    
 
-EVAL “convert_var_to_sinterval_tables ^only_var_table1 ^policy1_me1  ^test_pd_type1”;   
+val convert_to_interval1 = EVAL “convert_var_to_sinterval_tables ^only_var_table1 ^policy1_me1  ^test_pd_type1”;   
+
+
+val only_interval_table1 = optionSyntax.dest_some(rhs (concl convert_to_interval1));
+
+
+
+     
+val convert_var_to_sinterval_tables1_thm =
+REWRITE_RULE [] (ISPECL[only_var_table1, only_interval_table1, “0:num”, policy1_me1, test_pd_type1 ] correct_tables_from_var_to_sinterval_thm);        
+
+
+
+val final_table1_thm = SIMP_RULE bool_ss [convert_to_interval1] convert_var_to_sinterval_tables1_thm;    
+
+
+
+
+
+
+Definition mv_from_me_and_packet_def:
+  mv_from_me_and_packet me packet_input =
+  MAP (\(x,arith_atom). 
+        case eval_arithm_atom packet_input arith_atom of
+          NONE => NONE
+        | SOME v => SOME (x, v)
+      ) me
+End
+
+Definition create_mv_def:
+  create_mv me packet_input =
+  let all = mv_from_me_and_packet me packet_input in
+    let filtered = FILTER IS_SOME all in
+      MAP THE filtered
+End
+                                     
+ 
+
+
+Definition every_lval_in_me_in_type_def:
+  every_lval_in_me_in_type pd_type me =
+   EVERY (\(x,atom).  case (get_lval_from_arith atom) of
+                      | is_lval lval => (case resolve_lval_type pd_type lval of
+                                         | SOME (type_length n) => T
+                                         | _ => F ) 
+                      | _ => T) me                      
+End
+
+
+
+Definition ops_in_me_length_format_def:
+  ops_in_me_length_format pd_type me =
+  EVERY (\(x,atom).  case atom of
+                     | a_True => T
+                     | a_False => F           
+                     | arithm_ge lval m => (case resolve_lval_type pd_type lval of
+                                            | SOME (type_length n) => (n = SND m) 
+                                            | _ => F )
+                     | arithm_le lval m => (case resolve_lval_type pd_type lval of
+                                            | SOME (type_length n) => (n = SND m) 
+                                            | _ => F ) 
+        ) me                      
+End
+     
+
+     
+    
+Theorem lval_in_me_distinct_imp_cond1:
+∀ me pd_type packet_input .
+  ALL_DISTINCT (MAP FST me) ∧
+  every_lval_in_me_in_type pd_type me ⇒
+  (∀var atom.
+     ALOOKUP me var = SOME atom ⇒
+     ALOOKUP (create_mv me packet_input) var = eval_arithm_atom packet_input atom)
+Proof
+Induct >>
+rpt strip_tac >>
+gvs[create_mv_def] >>                 
+rw[mv_from_me_and_packet_def] >|[
+    PairCases_on ‘h’ >> gvs[] >>
+    rpt (BasicProvers.FULL_CASE_TAC >> gvs[]) >>
+    gvs[every_lval_in_me_in_type_def] >>
+    res_tac >>
+    gvs[mv_from_me_and_packet_def]
+    ,
+    PairCases_on ‘h’ >> gvs[] >>
+    rpt (BasicProvers.FULL_CASE_TAC >> gvs[]) >|[
+        simp[ALOOKUP_NONE] >>
+        gvs[MEM_MAP] >>
+        rpt strip_tac >>
+        gvs[MEM_FILTER] >>
+        gvs[MEM_MAP] >>
+        PairCases_on ‘y’ >> gvs[] >>
+        rpt (BasicProvers.FULL_CASE_TAC >> gvs[])
+                           
+        ,
+        gvs[every_lval_in_me_in_type_def] >>
+        res_tac >>
+        gvs[mv_from_me_and_packet_def]    
+      ]
+  ]
+QED
+         
+                             
+val every_lval_in_me_in_type_thm = EVAL “every_lval_in_me_in_type ^test_pd_type1 ^policy1_me1”;
+val all_distinct_fst_me_thm = EVAL “ALL_DISTINCT (MAP FST ^policy1_me1)”;
+
+val cond1_thm = REWRITE_RULE [every_lval_in_me_in_type_thm, all_distinct_fst_me_thm] (ISPECL[policy1_me1, test_pd_type1 ] lval_in_me_distinct_imp_cond1);   
+
+
+
+  
+Definition mv_dom_vars_exec_def:
+  mv_dom_vars_exec mv vars =
+  EVERY (\x. ALOOKUP mv x ≠ NONE) vars
+End
+
+Theorem lookup_is_some_not_none_eq:
+  ∀ mv x.
+    lookup_is_some mv x ⇔ ALOOKUP mv x ≠ NONE
+Proof
+  Induct >>
+  gvs[lookup_is_some_def] >>
+  rpt strip_tac >>
+  EQ_TAC >>
+  rpt strip_tac >>
+  gvs[] >>
+  Cases_on ‘ALOOKUP (h::mv) x’ >> gvs[]
+QED                  
+                                 
+        
+Theorem mv_dom_vars_exec_eq:
+  ∀ mv vars.
+    mv_dom_vars mv vars = mv_dom_vars_exec mv vars
+Proof
+  rw[mv_dom_vars_def, mv_dom_vars_exec_def] >>
+  gvs[EVERY_MEM, lookup_is_some_not_none_eq]
+QED
+
+
+
+Definition in_order_then_in_me_def:
+  in_order_then_in_me order me =
+  EVERY (\x. ALOOKUP me x ≠ NONE) order
+End
+
+
+
+Theorem wf_format_imp_cond2:
+  ∀ me pd_type order.
+    ∀ packet_input.
+      in_order_then_in_me order me ∧
+      ops_in_me_length_format pd_type me ∧
+      wf_packet pd_type packet_input ∧
+      ALL_DISTINCT (MAP FST me) ∧
+      every_lval_in_me_in_type pd_type me ⇒
+      mv_dom_vars (create_mv me packet_input) order
+Proof
+  rw[in_order_then_in_me_def] >>
+  gvs[mv_dom_vars_exec_eq] >>
+  gvs[mv_dom_vars_exec_def] >>
+  gvs[EVERY_MEM] >>
+  rpt strip_tac >>
+  res_tac >>
+  
+  
+  Cases_on ‘ALOOKUP me x’ >> gvs[] >>
+  imp_res_tac MEM_ALOOKUP_DISTINCT >>
+  
+  gvs[every_lval_in_me_in_type_def] >>
+  gvs[EVERY_MEM] >>
+  
+  res_tac >>
+  gvs[create_mv_def] >>
+  gvs[mv_from_me_and_packet_def] >>         
+  gvs[ALOOKUP_NONE] >>
+  gvs[MEM_MAP] >>
+  gvs[MEM_FILTER] >>
+  gvs[MEM_MAP] >>
+  
+  first_x_assum (strip_assume_tac o (Q.SPECL [‘(x,THE (eval_arithm_atom packet_input x'))’])) >> gvs[] >>
+  first_x_assum (strip_assume_tac o (Q.SPECL [‘SOME (x,THE (eval_arithm_atom packet_input x'))’])) >> gvs[] >>
+  first_x_assum (strip_assume_tac o (Q.SPECL [‘(x,x')’])) >> gvs[] >>
+  
+  rpt (BasicProvers.FULL_CASE_TAC >> gvs[]) >>
+  
+  Cases_on ‘x'’ >> 
+  gvs[eval_arithm_atom_def] >>
+  
+  rpt (BasicProvers.FULL_CASE_TAC >> gvs[]) >>
+  (* le and ge same proof *)
+  (
+  (* first and third subgoals *)
+  res_tac >>
+  fs[get_lval_from_arith_def] >>
+  rpt (BasicProvers.FULL_CASE_TAC >> gvs[]) >>
+  gvs[wf_packet_def] >>
+  res_tac >> gvs[] >>
+  
+  (* reach here only for second subgoal *)
+  
+  PairCases_on ‘bs’ >>
+  PairCases_on ‘y’ >>
+  PairCases_on ‘y'’ >>
+  gvs[] >>
+  
+  imp_res_tac MEM_ALOOKUP_DISTINCT >>
+  gvs[] >>
+  
+  gvs[ops_in_me_length_format_def] >>
+  gvs[EVERY_MEM] >>
+  res_tac >>
+  fs[] >>
+  
+  gvs[] >>
+  
+  PairCases_on ‘p’ >> gvs[] >>
+  imp_res_tac last_edge_of_binpred_neg >> gvs[]
+  )
+QED
+
+
+
+
+
+
+
+
+              
+val in_order_then_in_me_thm = EVAL “in_order_then_in_me ^policy1_order ^policy1_me1”;
+val ops_in_me_length_format_thm = EVAL “ops_in_me_length_format ^test_pd_type1 ^policy1_me1”;
+
+val cond2_thm = REWRITE_RULE [every_lval_in_me_in_type_thm, all_distinct_fst_me_thm,
+                             in_order_then_in_me_thm, ops_in_me_length_format_thm]
+                             (ISPECL[policy1_me1, test_pd_type1, policy1_order ]
+                                    wf_format_imp_cond2);   
+
+
+                                        
+
+
+
+
+Theorem create_mv_all_distinct:
+  ∀ me packet_input.
+    ALL_DISTINCT (MAP FST me) ⇒ ALL_DISTINCT (MAP FST (create_mv me packet_input))
+Proof
+  Induct >>
+  gvs[create_mv_def] >>
+  gvs[mv_from_me_and_packet_def] >>   
+  rpt strip_tac >>
+  
+  PairCases_on ‘h’ >> gvs[] >>
+  rpt (BasicProvers.FULL_CASE_TAC >> gvs[]) >>
+  
+  gvs[MEM_MAP, MEM_FILTER] >>
+  rpt strip_tac >>
+  Cases_on ‘y'’ >> gvs[] >>
+  rpt strip_tac >>
+  PairCases_on ‘y’ >> gvs[] >>
+  rpt (BasicProvers.FULL_CASE_TAC >> gvs[])
+QED
+                                              
+
+                                        
+Theorem create_mv_normalization:
+  ∀ h me packet_input.
+  create_mv (h::me) packet_input = (create_mv [h] packet_input)++(create_mv me packet_input)
+Proof
+  rw[create_mv_def] >>
+  gvs[mv_from_me_and_packet_def] >>
+  rpt (BasicProvers.FULL_CASE_TAC >> gvs[])
+QED
+
+
+Theorem ops_in_me_length_format_normalization:
+  ∀ h me pd_type.
+    ops_in_me_length_format pd_type (h::me) = (ops_in_me_length_format pd_type [h] ∧
+                                               ops_in_me_length_format pd_type me)
+Proof
+  rw[ops_in_me_length_format_def]
+QED
+
+
+        
+Theorem every_lval_in_me_in_type_normalization:
+  ∀ h me pd_type.
+    every_lval_in_me_in_type pd_type (h::me) = (every_lval_in_me_in_type pd_type [h] ∧
+                                                every_lval_in_me_in_type pd_type me )
+Proof
+  rw[every_lval_in_me_in_type_def]
+QED
+
+        
+                               
+Theorem if_in_create_mv_then_in_me:                                  
+  ∀ me var y.
+    ∀ packet_input.
+      ALL_DISTINCT (MAP FST me) ∧
+      ALOOKUP (create_mv me packet_input) var = SOME y ⇒
+      ∃y'. ALOOKUP me var = SOME y'
+Proof
+  Induct >>
+  rw[] >-
+   gvs[create_mv_def, mv_from_me_and_packet_def] >>
+  
+  imp_res_tac create_mv_all_distinct >>
+  first_x_assum (strip_assume_tac o (Q.SPECL [‘packet_input’])) >> 
+  
+  gvs[Once create_mv_normalization] >>
+  gvs[ALOOKUP_APPEND] >>
+  rpt (BasicProvers.FULL_CASE_TAC >> gvs[]) >|[
+    res_tac >>
+    PairCases_on ‘h’ >> gvs[] >>
+    BasicProvers.FULL_CASE_TAC >> gvs[]
+    ,
+    PairCases_on ‘h’ >> gvs[] >>
+    BasicProvers.FULL_CASE_TAC >> gvs[] >>
+    gvs[create_mv_def, mv_from_me_and_packet_def] >>
+    rpt (BasicProvers.FULL_CASE_TAC >> gvs[])
+  ]
+QED
+
+
+
+        
+Theorem wf_format_and_fail_create_single:
+  ∀ pd_type h var.
+    ∀ packet_input.
+      ops_in_me_length_format pd_type [h] ∧
+      wf_packet pd_type packet_input ∧
+      every_lval_in_me_in_type pd_type [h]  ∧
+      wf_packet pd_type packet_input ∧
+      ALOOKUP (create_mv [h] packet_input) var = NONE ⇒
+      FST h ≠ var
+Proof
+  
+  rw[create_mv_def] >>
+  gvs[mv_from_me_and_packet_def] >>
+  PairCases_on ‘h’ >> gvs[] >>
+  rpt (BasicProvers.FULL_CASE_TAC >> gvs[]) >>
+  gvs[every_lval_in_me_in_type_def] >>
+  
+  
+  Cases_on ‘h1’ >>
+  gvs[eval_arithm_atom_def] >>
+  rpt (BasicProvers.FULL_CASE_TAC >> gvs[]) >>
+  
+  
+  gvs[get_lval_from_arith_def] >>
+  
+  gvs[wf_packet_def] >>      
+  res_tac >>
+  gvs[] >>
+  
+  gvs[ops_in_me_length_format_def] >>
+  PairCases_on ‘p’ >> gvs[] >>
+  PairCases_on ‘bs’ >> gvs[] >>
+  imp_res_tac last_edge_of_binpred_neg >> gvs[]
+QED
+
+
+
+
+
+Theorem if_in_me_then_in_create_mv:                                  
+  ∀ me pd_type var y.
+    ∀ packet_input.
+      ops_in_me_length_format pd_type me ∧
+      wf_packet pd_type packet_input ∧
+      ALL_DISTINCT (MAP FST me) ∧
+      every_lval_in_me_in_type pd_type me ∧
+      ALOOKUP me var = SOME y
+      ⇒
+      ∃y'. ALOOKUP (create_mv me packet_input) var = SOME y'
+Proof
+
+  Induct >-
+   rw[] >>
+  rpt strip_tac >>
+  
+  imp_res_tac create_mv_all_distinct >>
+  first_x_assum (strip_assume_tac o (Q.SPECL [‘packet_input’])) >> 
+  
+  gvs[Once create_mv_normalization] >>
+  simp[Once create_mv_normalization] >>
+  
+  gvs[ALOOKUP_APPEND] >>
+  rpt (BasicProvers.FULL_CASE_TAC >> gvs[]) >>
+  
+  rgs[Once ops_in_me_length_format_normalization] >>
+  rgs[Once every_lval_in_me_in_type_normalization] >>
+  
+  res_tac >>
+  
+  imp_res_tac wf_format_and_fail_create_single >>
+  PairCases_on ‘h’ >> gvs[] >>
+  res_tac >> gvs[]
+QED
+              
+
+
+
+Theorem wf_format_imp_cond3:                                        
+  ∀ me pd_type.
+    ∀ packet_input.
+      ops_in_me_length_format pd_type me ∧
+      wf_packet pd_type packet_input ∧
+      ALL_DISTINCT (MAP FST me) ∧
+      every_lval_in_me_in_type pd_type me ⇒
+      (∀var. lookup_is_some (create_mv me packet_input) var ⇔
+               lookup_is_some me var)
+Proof
+  rw[lookup_is_some_def] >>
+  EQ_TAC >> strip_tac >|[
+    imp_res_tac if_in_create_mv_then_in_me >> gvs[]
+    ,
+    imp_res_tac if_in_me_then_in_create_mv >> gvs[]
+  ]
+QED
+
+
+   
+
+val cond3_thm = REWRITE_RULE [every_lval_in_me_in_type_thm, all_distinct_fst_me_thm,
+                             in_order_then_in_me_thm, ops_in_me_length_format_thm]
+                             (ISPECL[policy1_me1, test_pd_type1]
+                                    wf_format_imp_cond3);   
+
+
+
+
+
+    
+val final_thm = prove(
+“! packet_input .
+ wf_packet ^test_pd_type1 packet_input ⇒ 
+ sem_arith_policy ^arith_policy1 packet_input = 
+ sem_sinterval_tables (^only_interval_table1,0) packet_input”
+,
+
+rpt strip_tac >>
+assume_tac arith_policy1_var_policy1_thm >>
+first_x_assum (strip_assume_tac o (Q.SPECL [‘packet_input’,‘(create_mv ^policy1_me1 packet_input)’])) >>
+
+gvs[cond1_thm] >>
+
+assume_tac policy1_thm >>
+first_x_assum (strip_assume_tac o (Q.SPECL [‘(create_mv ^policy1_me1 packet_input)’])) >>
+
+imp_res_tac cond2_thm >>
+gvs[] >>
+          
+assume_tac final_table1_thm >>
+first_x_assum (strip_assume_tac o (Q.SPECL [‘packet_input’,‘(create_mv ^policy1_me1 packet_input)’])) >>
+gvs[cond1_thm] >>
+
+gvs[cond3_thm]
+);
+
+
+
+
+
+
+
+
+
+
+
+
+
+
+
+
 
              
-val convert_var_to_sinterval_tables1_thm =
-REWRITE_RULE [] (ISPECL[only_var_table1] correct_tables_from_var_to_sinterval_thm);        
-
-
-
-
-
-
     
-    
-
+(*
                                 
 (****************************************************************)
 (****************************************************************)
@@ -223,7 +699,7 @@ val policy2_thm_init = computeLib.RESTR_EVAL_CONV [“sem_tables”,“sem_polic
 val policy2_thm = SIMP_RULE bool_ss [correct_var_policy_var_tables_exec_thm1] policy2_thm_init;     
 
 
-
+*)
 
 
 
